share/pulse/examples/dice/cbor/CDDL.Spec.MapGroupGen2.Base.fst
@@ -1,0 +1,1397 @@
+module CDDL.Spec.MapGroupGen2.Base
+
+module FE = FStar.FunctionalExtensionality
+
+let cbor_map = ghost_map Cbor.raw_data_item Cbor.raw_data_item
+
+let map_group_item : Type0 =
+  (cbor_map & cbor_map)
+
+noeq
+type map_group_sem_result =
+| MapGroupResult of FStar.GSet.set map_group_item
+| MapGroupCutFailure
+
+let map_group_post'
+  (l: cbor_map)
+  (res: FStar.GSet.set map_group_item)
+: Tot prop
+=
+      forall l' .
+      FStar.GSet.mem l' res ==>  map_group_item_post l l'
+
+let map_group_post
+  (l: cbor_map)
+  (res: map_group_sem_result)
+: Tot prop
+= match res with
+  | MapGroupResult res -> map_group_post' l res
+  | MapGroupCutFailure -> True
+
+let map_group_codom
+  (l: cbor_map)
+: Tot Type0
+= (res: map_group_sem_result {
+      map_group_post l res
+  })
+
+let map_group : Type0 =
+  FE.restricted_g_t
+    (cbor_map)
+    (map_group_codom)
+
+let map_group_always_false : map_group =
+  FE.on_dom_g cbor_map #map_group_codom
+    (fun _ -> MapGroupResult FStar.GSet.empty)
+
+let map_group_nop : map_group =
+  FE.on_dom_g cbor_map #map_group_codom
+    (fun l -> MapGroupResult (FStar.GSet.singleton (ghost_map_empty, l)))
+
+let ghost_map_is_empty
+  (#key #value: Type)
+  (m: ghost_map key value)
+: Ghost bool
+  (requires True)
+  (ensures fun res -> res == true <==> m == ghost_map_empty)
+= FStar.StrongExcludedMiddle.strong_excluded_middle (m == ghost_map_empty)
+
+let map_group_end : map_group =
+  FE.on_dom_g cbor_map #map_group_codom
+    (fun l -> if ghost_map_is_empty l then map_group_nop l else map_group_always_false l)
+
+unfold
+let map_group_match_item_witness_pred (key value: typ) (l: cbor_map) (l': cbor_map & cbor_map) (x: Cbor.raw_data_item & Cbor.raw_data_item) : Tot prop =
+  map_group_item_post l l' /\
+  fst l' == ghost_map_singleton (fst x) (snd x) /\
+  key (fst x) /\
+  value (snd x)
+
+let pred2_equiv_trans
+  (#t #t': Type)
+  (p1 p2 p3: t -> t' -> prop)
+: Lemma
+  (requires (
+    (forall x x' . p1 x x' <==> p2 x x') /\
+    (forall x x' . p2 x x' <==> p3 x x')
+  ))
+  (ensures (
+    (forall x x' . p1 x x' <==> p3 x x')
+  ))
+= ()
+
+let map_group_match_item_comprehend
+  (key value: typ)
+  (l: cbor_map)
+  l'
+: GTot bool
+=
+    FStar.StrongExcludedMiddle.strong_excluded_middle (exists x .
+      map_group_match_item_witness_pred key value l l' x
+    )
+
+let map_group_match_item' (key value: typ) (l: cbor_map) : FStar.GSet.set map_group_item =
+  FStar.GSet.comprehend (map_group_match_item_comprehend key value l)
+
+let map_group_match_item_elim (key value: typ) (l: cbor_map) l' : Ghost _
+  (requires (FStar.GSet.mem l' (map_group_match_item' key value l)))
+  (ensures (fun x -> map_group_match_item_witness_pred key value l l' x))
+= FStar.IndefiniteDescription.indefinite_description_ghost _ (map_group_match_item_witness_pred key value l l')
+
+let map_group_match_item_cut_failure_witness_pred (key: typ) (s: FStar.GSet.set map_group_item) (l': (map_group_item & (Cbor.raw_data_item & Cbor.raw_data_item))) : Tot prop =
+  let (elt, entry) = l' in
+  let (_, rem) = elt in
+  let (k, _) = entry in
+  FStar.GSet.mem elt s /\
+  ghost_map_mem entry rem /\
+  key k
+
+let maybe_indefinite_description_ghost (#t: Type) (p: t -> prop) : Ghost (option t)
+  (requires True)
+  (ensures fun res ->
+    (Some? res <==> (exists l . p l)) /\
+    begin match res with
+    | None -> True
+    | Some l -> p l
+    end
+  )
+= if FStar.StrongExcludedMiddle.strong_excluded_middle (exists l . p l)
+  then Some (FStar.IndefiniteDescription.indefinite_description_ghost _ p)
+  else None
+
+#restart-solver
+let gset_is_empty
+  (#t: Type)
+  (s: FStar.GSet.set t)
+: Ghost (option t)
+    (requires True)
+    (ensures fun res -> 
+    (None? res <==> s == FStar.GSet.empty) /\
+    begin match res with
+    | None -> True
+    | Some x -> FStar.GSet.mem x s
+    end
+    )
+= match maybe_indefinite_description_ghost (fun x -> FStar.GSet.mem x s) with
+  | Some x -> Some x
+  | None ->
+    assert (s `FStar.GSet.equal` FStar.GSet.empty);
+    None
+
+let map_group_match_item_cut_pre
+  (l: cbor_map)
+  (s: FStar.GSet.set map_group_item)
+: GTot (FStar.GSet.set map_group_item)
+= 
+    match gset_is_empty s with
+    | None -> FStar.GSet.singleton (ghost_map_empty, l)
+    | _ -> s
+
+let map_group_match_item_cut
+  (key: typ)
+  (l: cbor_map)
+  (s: FStar.GSet.set map_group_item)
+: GTot map_group_sem_result
+= 
+  let s' = map_group_match_item_cut_pre l s in
+  match maybe_indefinite_description_ghost (map_group_match_item_cut_failure_witness_pred key s') with
+  | Some _ -> MapGroupCutFailure
+  | _ -> MapGroupResult s
+
+let map_group_match_item (cut: bool) (key value: typ) : map_group =
+  FE.on_dom_g cbor_map #map_group_codom
+    (fun l ->
+      let s = map_group_match_item' key value l in
+      if cut
+      then map_group_match_item_cut key l s
+      else MapGroupResult s
+    )
+
+let gset_map_witness_pred (#t1 #t2: Type) (f: t1 -> GTot t2) (s: FStar.GSet.set t1) x2 x1 : GTot prop =
+  x2 == f x1 /\ FStar.GSet.mem x1 s
+
+let gset_map (#t1 #t2: Type) (f: t1 -> GTot t2) (s: FStar.GSet.set t1) : FStar.GSet.set t2 =
+  FStar.GSet.comprehend (fun x2 -> FStar.StrongExcludedMiddle.strong_excluded_middle (exists x1 .
+    gset_map_witness_pred f s x2 x1
+  ))
+
+let gset_map_elim #t1 #t2 (f: t1 -> GTot t2) (s: FStar.GSet.set t1) (x2: t2) : Ghost t1
+  (requires FStar.GSet.mem x2 (gset_map f s))
+  (ensures fun x1 -> gset_map_witness_pred f s x2 x1)
+= FStar.IndefiniteDescription.indefinite_description_ghost _ (gset_map_witness_pred f s x2)
+
+let map_group_match_item_alt_pred
+  (key value: typ)
+  (l: cbor_map)
+  (kv: (Cbor.raw_data_item & Cbor.raw_data_item))
+: Tot prop
+= ghost_map_mem kv l /\
+  matches_map_group_entry key value kv
+
+let map_group_match_item_alt_r
+  l0
+  (ll, lr)
+= (ll, ghost_map_union l0 lr)
+
+let map_group_match_item_alt (key value: typ) (l: cbor_map) : GTot _ =
+  match maybe_indefinite_description_ghost (map_group_match_item_alt_pred key value l) with
+  | None -> FStar.GSet.empty
+  | Some kv ->
+    let l1 = ghost_map_singleton (fst kv) (snd kv) in
+    let l2 = ghost_map_sub l l1 in
+    FStar.GSet.union (FStar.GSet.singleton (l1, l2))
+      (gset_map (map_group_match_item_alt_r l1) (map_group_match_item' key value l2))
+
+#restart-solver
+let map_group_match_item_alt_map_group_match_item
+  (key value: typ) (l: cbor_map) l'
+: Lemma
+  (FStar.GSet.mem l' (map_group_match_item_alt key value l) ==> FStar.GSet.mem l' (map_group_match_item' key value l))
+=
+  if FStar.GSet.mem l' (map_group_match_item_alt key value l)
+  then begin
+    let Some kv = maybe_indefinite_description_ghost (map_group_match_item_alt_pred key value l) in
+    let l1 = ghost_map_singleton (fst kv) (snd kv) in
+    let l2 = ghost_map_sub l l1 in
+    if FStar.StrongExcludedMiddle.strong_excluded_middle (l' == (l1, l2))
+    then assert (map_group_match_item_witness_pred key value l l' kv)
+    else begin
+      let x = gset_map_elim (map_group_match_item_alt_r l1) (map_group_match_item' key value l2) l' in
+      let kv' = map_group_match_item_elim key value l2 x in
+      ghost_map_union_assoc l1 (fst x) (snd x);
+      ghost_map_disjoint_union_comm l1 (fst x);
+      ghost_map_union_assoc (fst x) l1 (snd x);
+      assert (map_group_match_item_witness_pred key value l l' kv')
+    end
+  end
+
+let map_group_match_item_map_group_match_item_alt
+  (key value: typ) (l: cbor_map) l'
+: Lemma
+  (FStar.GSet.mem l' (map_group_match_item' key value l) ==> FStar.GSet.mem l' (map_group_match_item_alt key value l))
+= if FStar.GSet.mem l' (map_group_match_item' key value l)
+  then begin
+    let kv' = map_group_match_item_elim key value l l' in
+    assert (map_group_match_item_alt_pred key value l kv');
+    let Some kv = maybe_indefinite_description_ghost (map_group_match_item_alt_pred key value l) in
+    let l1 = ghost_map_singleton (fst kv) (snd kv) in
+    let l2 = ghost_map_sub l l1 in
+    if FStar.StrongExcludedMiddle.strong_excluded_middle (kv == kv')
+    then ghost_map_disjoint_union_simpl_l l1 l2 (snd l')
+    else begin
+      assert (ghost_map_mem kv' l2);
+      let l2' = snd l' `ghost_map_sub` l1 in
+      ghost_map_disjoint_union_comm l1 l2';
+      ghost_map_union_assoc (fst l') l1 l2';
+      ghost_map_disjoint_union_comm (fst l') l1;
+      ghost_map_union_assoc l1 (fst l') l2';
+      ghost_map_disjoint_union_simpl_l l1 (fst l' `ghost_map_union` l2') l2;
+      assert (map_group_match_item_witness_pred key value l2 (fst l', l2') kv');
+      assert (gset_map_witness_pred (map_group_match_item_alt_r l1) (map_group_match_item' key value l2) l' (fst l', l2'))
+    end
+  end
+
+let map_group_equiv
+  (m1 m2: map_group)
+: Tot prop
+= forall l . match m1 l, m2 l with
+  | MapGroupCutFailure, MapGroupCutFailure -> True
+  | MapGroupResult s1, MapGroupResult s2 -> s1 `FStar.GSet.equal` s2
+  | _ -> False
+
+let map_group_equiv_eq
+  (m1 m2: map_group)
+: Lemma
+  (map_group_equiv m1 m2 <==> m1 == m2)
+  [SMTPat (map_group_equiv m1 m2)]
+= assert (FE.feq_g m1 m2 <==> m1 == m2)
+
+let map_group_match_item_alt_correct
+  (key value: typ) (l: cbor_map)
+: Lemma
+  (map_group_match_item_alt key value l == map_group_match_item' key value l)
+= Classical.forall_intro (map_group_match_item_map_group_match_item_alt key value l);
+  Classical.forall_intro (map_group_match_item_alt_map_group_match_item key value l);
+  assert (map_group_match_item_alt key value l `FStar.GSet.equal` map_group_match_item' key value l)
+
+let map_group_choice (m1 m2: map_group) : map_group =
+  FE.on_dom_g cbor_map #map_group_codom (fun l ->
+    // greedy PEG semantics for `//`
+    match m1 l with
+    | MapGroupCutFailure -> MapGroupCutFailure
+    | MapGroupResult res1 ->
+      if FStar.StrongExcludedMiddle.strong_excluded_middle (res1 == FStar.GSet.empty)
+      then m2 l
+      else MapGroupResult res1
+  )
+
+let map_group_concat_witness_pred
+  (m1 m2: map_group)
+  (l: cbor_map)
+  (l': (cbor_map & cbor_map))
+  (l1l2: ((cbor_map & cbor_map) & (cbor_map & cbor_map)))
+: Tot prop
+= let (l1, l2) = l1l2 in
+  MapGroupResult? (m1 l) /\
+  FStar.GSet.mem l1 (MapGroupResult?._0 (m1 l)) /\
+  MapGroupResult? (m2 (snd l1)) /\
+  FStar.GSet.mem l2 (MapGroupResult?._0 (m2 (snd l1))) /\
+  fst l' `ghost_map_feq` (fst l1 `ghost_map_union` fst l2) /\
+  snd l' == snd l2
+
+let ghost_map_disjoint_union_elim
+  (#key #value: Type)
+  (m m1 m2: ghost_map key value)
+: Lemma
+  (requires ghost_map_disjoint m (m1 `ghost_map_union` m2))
+  (ensures ghost_map_disjoint m m1 /\ ghost_map_disjoint m m2)
+= ()
+
+let ghost_map_disjoint_union_intro
+  (#key #value: Type)
+  (m m1 m2: ghost_map key value)
+: Lemma
+  (requires ghost_map_disjoint m m1 /\ ghost_map_disjoint m m2)
+  (ensures ghost_map_disjoint m (m1 `ghost_map_union` m2))
+= ()
+
+#push-options "--z3rlimit 16"
+
+#restart-solver
+let map_group_concat_witness_pred_correct
+  (m1 m2: map_group)
+  (l: cbor_map)
+  (l': (cbor_map & cbor_map))
+  (l1l2: ((cbor_map & cbor_map) & (cbor_map & cbor_map)))
+: Lemma
+  (requires map_group_concat_witness_pred m1 m2 l l' l1l2)
+  (ensures map_group_item_post l l' /\
+    fst (fst l1l2) `ghost_map_disjoint` fst (snd l1l2))
+  [SMTPat (map_group_concat_witness_pred m1 m2 l l' l1l2)]
+= let (l1, l2) = l1l2 in
+  ghost_map_union_assoc (fst l1) (fst l2) (snd l2);
+  assert ((fst l1 `ghost_map_union` fst l2) `ghost_map_union` snd l2 == l);
+  assert (fst l1 `ghost_map_disjoint` snd l1);
+  assert (snd l1 == fst l2 `ghost_map_union` snd l2);
+  ghost_map_disjoint_union_elim (fst l1) (fst l2) (snd l2);
+  assert (fst l1 `ghost_map_disjoint` fst l2);
+  assert (fst l2 `ghost_map_disjoint` snd l2);
+  assert (ghost_map_disjoint (fst l1 `ghost_map_union` fst l2) (snd l2))
+
+#pop-options
+
+let map_group_concat_cut_failure_witness_pred
+  (m1 m2: map_group)
+  (l: cbor_map)
+  (l1: map_group_item)
+: Tot prop
+= MapGroupResult? (m1 l) /\
+  FStar.GSet.mem l1 (MapGroupResult?._0 (m1 l)) /\
+  MapGroupCutFailure? (m2 (snd l1))
+
+let map_group_concat (m1 m2: map_group) : map_group =
+  FE.on_dom_g cbor_map #map_group_codom
+    (fun l -> 
+      if MapGroupCutFailure? (m1 l)
+      then MapGroupCutFailure
+      else if FStar.StrongExcludedMiddle.strong_excluded_middle (exists l1 . map_group_concat_cut_failure_witness_pred m1 m2 l l1)
+      then MapGroupCutFailure
+      else MapGroupResult (
+        FStar.GSet.comprehend (fun l' -> FStar.StrongExcludedMiddle.strong_excluded_middle (exists l1l2 . map_group_concat_witness_pred m1 m2 l l' l1l2))
+    ))
+  
+let map_group_concat_elim (m1 m2: map_group) (l: cbor_map) l' : Ghost _
+  (requires (match map_group_concat m1 m2 l with
+  | MapGroupResult s -> FStar.GSet.mem l' s
+  | _ -> False
+  ))
+  (ensures fun l1l2 ->
+    map_group_concat_witness_pred m1 m2 l l' l1l2
+  )
+= FStar.IndefiniteDescription.indefinite_description_ghost _ (fun l1l2 -> map_group_concat_witness_pred m1 m2 l l' l1l2)
+
+let map_group_equiv_intro
+  (m1 m2: map_group)
+  (prf0: (l: cbor_map) -> Lemma (MapGroupCutFailure? (m1 l) == MapGroupCutFailure? (m2 l)))
+  (prf12: (l: cbor_map) ->
+    (l': _) ->
+    Lemma
+    (requires (match m1 l, m2 l with
+    | MapGroupResult s1, MapGroupResult _ -> FStar.GSet.mem l' s1
+    | _ -> False
+    ))
+    (ensures (match m2 l with
+    | MapGroupResult s2 -> FStar.GSet.mem l' s2
+    | _ -> True
+    ))
+  )
+  (prf21: (l: cbor_map) ->
+    (l': _) ->
+    Lemma
+    (requires (match m1 l, m2 l with
+    | MapGroupResult _, MapGroupResult s2 -> FStar.GSet.mem l' s2
+    | _ -> False
+    ))
+    (ensures (match m1 l with
+    | MapGroupResult s1 -> FStar.GSet.mem l' s1
+    | _ -> True
+    ))
+  )
+: Lemma
+  (map_group_equiv m1 m2)
+= Classical.forall_intro prf0;
+  Classical.forall_intro_2 (fun l l' -> Classical.move_requires (prf12 l) l');
+  Classical.forall_intro_2 (fun l l' -> Classical.move_requires (prf21 l) l')
+
+let map_group_equiv_intro_equiv
+  (m1 m2: map_group)
+  (prf0: (l: cbor_map) -> Lemma (MapGroupCutFailure? (m1 l) == MapGroupCutFailure? (m2 l)))
+  (prf: (l: cbor_map) ->
+    (l': _) ->
+    Lemma
+    (requires (
+      MapGroupResult? (m1 l) /\ MapGroupResult? (m2 l)
+    ))
+    (ensures (match m1 l, m2 l with
+    | MapGroupResult s1, MapGroupResult s2 -> (FStar.GSet.mem l' s1 <==> FStar.GSet.mem l' s2)
+    | _ -> True
+    ))
+  )
+: Lemma
+  (map_group_equiv m1 m2)
+= map_group_equiv_intro m1 m2 prf0 (fun l l' -> prf0 l; prf l l') (fun l l' -> prf0 l; prf l l')
+
+let map_group_equiv_intro_equiv_rec
+  (m1 m2: map_group)
+  (prf0: (l: cbor_map) -> 
+    (prf: (
+      (l1: cbor_map { ghost_map_length l1 < ghost_map_length l }) -> Lemma
+      (m1 l1 == m2 l1)
+    )) ->
+    Lemma (MapGroupCutFailure? (m1 l) == MapGroupCutFailure? (m2 l)))
+  (prf: (l: cbor_map) ->
+    (prf: (
+      (l1: cbor_map { ghost_map_length l1 < ghost_map_length l }) -> Lemma
+      (m1 l1 == m2 l1)
+    )) ->
+    (l': _) ->
+    Lemma
+    (requires (
+      MapGroupResult? (m1 l) /\ MapGroupResult? (m2 l)
+    ))
+    (ensures (match m1 l, m2 l with
+    | MapGroupResult s1, MapGroupResult s2 -> (FStar.GSet.mem l' s1 <==> FStar.GSet.mem l' s2)
+    | _ -> True
+    ))
+  )
+: Lemma
+  (map_group_equiv m1 m2)
+= let rec prf'
+      (l: cbor_map)
+  : Lemma
+      (ensures (m1 l == m2 l))
+      (decreases (ghost_map_length l))
+  = prf0 l prf';
+    match m1 l with
+    | MapGroupCutFailure -> ()
+    | MapGroupResult s1 ->
+      Classical.forall_intro (Classical.move_requires (prf l prf'));
+      assert (s1 `FStar.GSet.equal` MapGroupResult?._0 (m2 l))
+  in
+  map_group_equiv_intro_equiv m1 m2 (fun l -> prf' l) (fun l _ -> prf' l)
+
+let map_group_equiv_intro_rec
+  (m1 m2: map_group)
+  (prf0: (l: cbor_map) -> 
+    (prf: (
+      (l1: cbor_map { ghost_map_length l1 < ghost_map_length l }) -> Lemma
+      (m1 l1 == m2 l1)
+    )) ->
+    Lemma (MapGroupCutFailure? (m1 l) == MapGroupCutFailure? (m2 l)))
+  (prf12: (l: cbor_map) ->
+    (prf: (
+      (l1: cbor_map { ghost_map_length l1 < ghost_map_length l }) -> Lemma
+      (m1 l1 == m2 l1)
+    )) ->
+    (l': _) ->
+    Lemma
+    (requires (match m1 l, m2 l with
+    | MapGroupResult s1, MapGroupResult _ -> FStar.GSet.mem l' s1
+    | _ -> False
+    ))
+    (ensures (match m2 l with
+    | MapGroupResult s2 -> FStar.GSet.mem l' s2
+    | _ -> True
+    ))
+  )
+  (prf21: (l: cbor_map) ->
+    (prf: (
+      (l1: cbor_map { ghost_map_length l1 < ghost_map_length l }) -> Lemma
+      (m1 l1 == m2 l1)
+    )) ->
+    (l': _) ->
+    Lemma
+    (requires (match m1 l, m2 l with
+    | MapGroupResult _, MapGroupResult s2 -> FStar.GSet.mem l' s2
+    | _ -> False
+    ))
+    (ensures (match m1 l with
+    | MapGroupResult s1 -> FStar.GSet.mem l' s1
+    | _ -> True
+    ))
+  )
+: Lemma
+  (map_group_equiv m1 m2)
+= map_group_equiv_intro_equiv_rec m1 m2 prf0 (fun l prf l' ->
+    Classical.move_requires (prf12 l prf) l';
+    Classical.move_requires (prf21 l prf) l'
+  )
+
+let ghost_map_disjoint_union_assoc_domain
+  (#key #value: Type)
+  (f1 f2 f3: ghost_map key value)
+: Lemma
+  (ensures (
+    (f1 `ghost_map_disjoint` f2 /\ (f1 `ghost_map_union` f2) `ghost_map_disjoint` f3) <==>
+      (f2 `ghost_map_disjoint` f3 /\ f1 `ghost_map_disjoint` (f2 `ghost_map_union` f3))
+  ))
+= ()
+
+let ghost_map_disjoint_union_assoc
+  (#key #value: Type)
+  (f1 f2 f3: ghost_map key value)
+: Lemma
+  (requires
+      (f1 `ghost_map_disjoint` f2 /\ (f1 `ghost_map_union` f2) `ghost_map_disjoint` f3) \/
+      (f2 `ghost_map_disjoint` f3 /\ f1 `ghost_map_disjoint` (f2 `ghost_map_union` f3))
+  )
+  (ensures
+    (f1 `ghost_map_union` (f2 `ghost_map_union` f3) == (f1 `ghost_map_union` f2) `ghost_map_union` f3)
+  )
+= assert ((f1 `ghost_map_union` (f2 `ghost_map_union` f3)) `ghost_map_feq` ((f1 `ghost_map_union` f2) `ghost_map_union` f3))
+
+#push-options "--z3rlimit 32"
+
+#restart-solver
+let map_group_concat_assoc' (m1 m2 m3: map_group) : Lemma
+  (map_group_concat m1 (map_group_concat m2 m3) `map_group_equiv` map_group_concat (map_group_concat m1 m2) m3)
+= map_group_equiv_intro
+    (map_group_concat m1 (map_group_concat m2 m3))
+    (map_group_concat (map_group_concat m1 m2) m3)
+    (fun l -> match m1 l with
+    | MapGroupCutFailure -> ()
+    | MapGroupResult s1 ->
+      if FStar.StrongExcludedMiddle.strong_excluded_middle (exists l1 . map_group_concat_cut_failure_witness_pred m1 m2 l l1)
+      then
+        let l1 = FStar.IndefiniteDescription.indefinite_description_ghost _ (fun l1 -> map_group_concat_cut_failure_witness_pred m1 m2 l l1) in
+        assert (map_group_concat_cut_failure_witness_pred m1 (map_group_concat m2 m3) l l1)
+      else if FStar.StrongExcludedMiddle.strong_excluded_middle (exists l12 . map_group_concat_cut_failure_witness_pred (map_group_concat m1 m2) m3 l l12)
+      then
+        let l12 = FStar.IndefiniteDescription.indefinite_description_ghost _ (fun l12 -> map_group_concat_cut_failure_witness_pred (map_group_concat m1 m2) m3 l l12) in
+        let (l1, l2) = map_group_concat_elim m1 m2 l l12 in
+        assert (map_group_concat_cut_failure_witness_pred m2 m3 (snd l1) l2);
+        assert (map_group_concat_cut_failure_witness_pred m1 (map_group_concat m2 m3) l l1)
+      else if FStar.StrongExcludedMiddle.strong_excluded_middle (exists l1 . map_group_concat_cut_failure_witness_pred m1 (map_group_concat m2 m3) l l1)
+      then
+        let l1 = FStar.IndefiniteDescription.indefinite_description_ghost _ (fun l1 -> map_group_concat_cut_failure_witness_pred m1 (map_group_concat m2 m3) l l1) in
+        assert (MapGroupResult? (m2 (snd l1)));
+        let l2 = FStar.IndefiniteDescription.indefinite_description_ghost _ (fun l2 -> map_group_concat_cut_failure_witness_pred m2 m3 (snd l1) l2) in
+        let l12 = (fst l1 `ghost_map_union` fst l2, snd l2) in
+        assert (map_group_concat_witness_pred m1 m2 l l12 (l1, l2));
+        assert (map_group_concat_cut_failure_witness_pred (map_group_concat m1 m2) m3 l l12)
+      else ()
+    )
+    (fun l l' -> 
+      let (l1, l23) = map_group_concat_elim m1 (map_group_concat m2 m3) l l' in
+      ghost_map_disjoint_mem_union' (fst l1) (fst l23) ();
+      let (l2, l3) = map_group_concat_elim m2 m3 (snd l1) l23 in
+      ghost_map_disjoint_mem_union' (fst l2) (fst l3) ();
+      assert (FStar.GSet.mem l1 (MapGroupResult?._0 (m1 l)));
+      assert (FStar.GSet.mem l2 (MapGroupResult?._0 (m2 (snd l1))));
+      assert (FStar.GSet.mem l3 (MapGroupResult?._0 (m3 (snd l2))));
+      let l12 = (fst l1 `ghost_map_union` fst l2, snd l2) in
+      ghost_map_disjoint_mem_union' (fst l1) (fst l2) ();
+      assert (map_group_concat_witness_pred m1 m2 l l12 (l1, l2));
+      ghost_map_disjoint_union_assoc (fst l1) (fst l2) (fst l3);
+      ghost_map_disjoint_mem_union' (fst l12) (fst l3) ();
+      assert (map_group_concat_witness_pred (map_group_concat m1 m2) m3 l l' (l12, l3))
+    )
+    (fun l l' ->
+      let (l12, l3) = map_group_concat_elim (map_group_concat m1 m2) m3 l l' in
+      ghost_map_disjoint_mem_union' (fst l12) (fst l3) ();
+      let (l1, l2) = map_group_concat_elim m1 m2 l l12 in
+      ghost_map_disjoint_mem_union' (fst l1) (fst l2) ();
+      let l23 = (fst l2 `ghost_map_union` fst l3, snd l3) in
+      ghost_map_disjoint_mem_union' (fst l2) (fst l3) ();
+      assert (map_group_concat_witness_pred m2 m3 (snd l1) l23 (l2, l3));
+      ghost_map_disjoint_union_assoc (fst l1) (fst l2) (fst l3);
+      ghost_map_disjoint_mem_union' (fst l1) (fst l23) ();
+      assert (map_group_concat_witness_pred m1 (map_group_concat m2 m3) l l' (l1, l23))
+    )
+
+#pop-options
+
+let map_group_concat_assoc m1 m2 m3 =
+  map_group_concat_assoc' m1 m2 m3
+
+#restart-solver
+let map_group_concat_nop_l
+  (m: map_group)
+: Lemma
+  (map_group_concat map_group_nop m == m)
+= map_group_equiv_intro
+    (map_group_concat map_group_nop m)
+    m
+    (fun l -> match m l with
+    | MapGroupCutFailure -> assert (map_group_concat_cut_failure_witness_pred map_group_nop m l (ghost_map_empty, l))
+    | MapGroupResult _ -> ()
+    )
+    (fun l l' ->
+      let (l1, l2) = map_group_concat_elim map_group_nop m l l' in
+      assert (fst l' `ghost_map_feq` fst l2)
+    )
+    (fun l l' ->
+      assert (map_group_concat_witness_pred map_group_nop m l l' ((ghost_map_empty, l), l'))
+    )
+
+let map_group_concat_nop_r
+  (m: map_group)
+: Lemma
+  (map_group_concat m map_group_nop == m)
+= map_group_equiv_intro
+    (map_group_concat m map_group_nop)
+    m
+    (fun _ -> ())
+    (fun l l' ->
+      let (l1, l2) = map_group_concat_elim m map_group_nop l l' in
+      assert (fst l' `ghost_map_feq` fst l1)
+    )
+    (fun l l' -> 
+      assert (map_group_concat_witness_pred m map_group_nop l l' (l', (ghost_map_empty, snd l')))
+    )
+
+let bound_map_group
+  (l0: cbor_map)
+  (m: (l: cbor_map { ghost_map_length l < ghost_map_length l0 }) ->
+  Ghost _
+    (requires True)
+    (ensures fun l' -> map_group_post l l')
+  )
+: map_group
+= FE.on_dom_g cbor_map #map_group_codom
+    (fun l -> if ghost_map_length l >= ghost_map_length l0 then map_group_nop l else m l)
+
+let bound_map_group_ext
+  (l0: cbor_map)
+  (m1 m2: (l: cbor_map { ghost_map_length l < ghost_map_length l0 }) ->
+  Ghost _
+    (requires True)
+    (ensures fun l' -> map_group_post l l')
+  )
+: Lemma
+  (requires forall (l: cbor_map { ghost_map_length l < ghost_map_length l0 }) .
+    m1 l == m2 l
+  )
+  (ensures bound_map_group l0 m1 == bound_map_group l0 m2)
+= map_group_equiv_intro (bound_map_group l0 m1) (bound_map_group l0 m2)
+    (fun l -> ())
+    (fun l l' -> ())
+    (fun l l' -> ())
+
+// greedy PEG semantics for `*`
+let rec map_group_zero_or_more'
+  (m: map_group)
+  (l: cbor_map)
+: GTot (l': _ {
+    map_group_post l l'
+  })
+  (decreases (ghost_map_length l))
+= match m l with
+  | MapGroupCutFailure -> MapGroupCutFailure
+  | MapGroupResult res1 ->
+    if FStar.StrongExcludedMiddle.strong_excluded_middle (res1 == FStar.GSet.empty)
+    then map_group_nop l
+    else map_group_concat m (bound_map_group l (map_group_zero_or_more' m)) l
+
+let map_group_zero_or_more m =
+  FE.on_dom_g cbor_map #map_group_codom (map_group_zero_or_more' m)
+
+let map_group_zero_or_more_eq
+  (m: map_group)
+  (l: cbor_map)
+: Lemma
+  (ensures (map_group_zero_or_more m l == (match m l with
+  | MapGroupCutFailure -> MapGroupCutFailure
+  | MapGroupResult res1 ->
+    if FStar.StrongExcludedMiddle.strong_excluded_middle (res1 == FStar.GSet.empty)
+    then map_group_nop l
+    else map_group_concat m (bound_map_group l (map_group_zero_or_more m)) l
+  )))
+  (decreases (ghost_map_length l))
+= assert (forall l . map_group_zero_or_more m l == map_group_zero_or_more' m l);
+  assert_norm (map_group_zero_or_more' m l == (match m l with
+  | MapGroupCutFailure -> MapGroupCutFailure
+  | MapGroupResult res1 ->
+    if FStar.StrongExcludedMiddle.strong_excluded_middle (res1 == FStar.GSet.empty)
+    then map_group_nop l
+    else map_group_concat m (bound_map_group l (map_group_zero_or_more' m)) l
+  ));
+  bound_map_group_ext l (map_group_zero_or_more m) (map_group_zero_or_more' m)
+
+#restart-solver
+let map_group_match_item_for_eq_none
+  (cut: bool)
+  (k: Cbor.raw_data_item)
+  (ty: typ)
+  (l: cbor_map)
+: Lemma
+  (requires (
+    ~ (ghost_map_defined k l)
+  ))
+  (ensures (
+    map_group_match_item_for cut k ty l == MapGroupResult FStar.GSet.empty
+  ))
+= map_group_match_item_alt_correct (t_literal k) ty l
+
+#restart-solver
+let map_group_match_item_for_eq
+  (k: Cbor.raw_data_item)
+  (ty: typ)
+  (l: cbor_map)
+: Lemma
+  (ensures (
+    map_group_match_item_for false k ty l == begin match apply_ghost_map l k with
+    | Some v ->
+      if ty v
+      then
+        let s = ghost_map_singleton k v in
+        MapGroupResult (FStar.GSet.singleton (s, l `ghost_map_sub` s))
+      else
+        MapGroupResult FStar.GSet.empty
+    | _ -> MapGroupResult FStar.GSet.empty
+    end
+  ))
+= map_group_match_item_alt_correct (t_literal k) ty l;
+  match maybe_indefinite_description_ghost (map_group_match_item_alt_pred (t_literal k) ty l) with
+  | None ->
+    begin match apply_ghost_map l k with
+    | None -> ()
+    | Some v -> if ty v
+      then assert (map_group_match_item_alt_pred (t_literal k) ty l (k, v))
+      else ()
+    end
+  | Some (k', v) ->
+    assert (k == k');
+    assert (apply_ghost_map l k == Some v);
+    let l1 = ghost_map_singleton k v in
+    let l2 = l `ghost_map_sub` l1 in
+    map_group_match_item_for_eq_none false k ty l2;
+    assert (FStar.GSet.equal
+      (gset_map (map_group_match_item_alt_r l1) (map_group_match_item' (t_literal k) ty l2))
+      FStar.GSet.empty
+    );
+    assert (FStar.GSet.equal
+      (FStar.GSet.singleton (l1, l2) `FStar.GSet.union` FStar.GSet.empty)
+      (FStar.GSet.singleton (l1, l2))
+    )
+
+#restart-solver
+let map_group_match_item_for_eq_gen
+  (cut: bool)
+  (k: Cbor.raw_data_item)
+  (ty: typ)
+  (l: cbor_map)
+: Lemma
+  (ensures (
+    map_group_match_item_for cut k ty l == begin match apply_ghost_map l k with
+    | Some v ->
+      if ty v
+      then
+        let s = ghost_map_singleton k v in
+        MapGroupResult (FStar.GSet.singleton (s, l `ghost_map_sub` s))
+      else if cut
+      then MapGroupCutFailure
+      else
+        MapGroupResult FStar.GSet.empty
+    | _ -> MapGroupResult FStar.GSet.empty
+    end
+  ))
+= map_group_match_item_for_eq k ty l;
+  if cut
+  then match apply_ghost_map l k with
+  | None -> ()
+  | Some v ->
+    let l1 = ghost_map_singleton k v in
+    let l2 = l `ghost_map_sub` l1 in
+    if ty v
+    then match maybe_indefinite_description_ghost (map_group_match_item_cut_failure_witness_pred (t_literal k) (FStar.GSet.singleton (l1, l2))) with
+    | None -> ()
+    | Some _ -> assert False
+    else begin
+      assert (map_group_match_item_for false k ty l == MapGroupResult FStar.GSet.empty);
+      assert (None? (gset_is_empty #map_group_item FStar.GSet.empty));
+      assert (map_group_match_item_cut_pre l FStar.GSet.empty == FStar.GSet.singleton (ghost_map_empty, l));
+      assert (map_group_match_item_cut_failure_witness_pred (t_literal k) (FStar.GSet.singleton (ghost_map_empty, l)) ((ghost_map_empty, l), (k, v)));
+      assert (Some? (maybe_indefinite_description_ghost (map_group_match_item_cut_failure_witness_pred (t_literal k) (FStar.GSet.singleton (ghost_map_empty, l)))));
+      assert (map_group_match_item_for true k ty l == MapGroupCutFailure)
+    end
+
+let gset_equal_intro
+  (#t: Type)
+  (s1 s2: FStar.GSet.set t)
+  (prf12: (x: t) -> Lemma
+    (requires FStar.GSet.mem x s1)
+    (ensures FStar.GSet.mem x s2)
+  )
+  (prf21: (x: t) -> Lemma
+    (requires FStar.GSet.mem x s2)
+    (ensures FStar.GSet.mem x s1)
+  )
+: Lemma
+  (s1 == s2)
+= Classical.forall_intro (Classical.move_requires prf12);
+  Classical.forall_intro (Classical.move_requires prf21);
+  assert (s1 `FStar.GSet.equal` s2)
+
+let map_group_match_item_length
+  (key value: typ)
+  (l: cbor_map)
+  l'
+: Lemma
+  (requires FStar.GSet.mem l' (map_group_match_item' key value l))
+  (ensures ghost_map_length (snd l') < ghost_map_length l)
+  [SMTPat (FStar.GSet.mem l' (map_group_match_item' key value l))]
+= ()
+
+#restart-solver
+let map_group_zero_or_more_zero_or_one_eq
+  (m: map_group)
+: Lemma
+  (map_group_zero_or_more (map_group_zero_or_one m) == map_group_zero_or_more m)
+=
+  assert ((ghost_map_empty #Cbor.raw_data_item #Cbor.raw_data_item  `ghost_map_union` ghost_map_empty) `ghost_map_feq` ghost_map_empty);
+  map_group_equiv_intro_rec
+    (map_group_zero_or_more (map_group_zero_or_one m))
+    (map_group_zero_or_more m)
+    (fun l prf ->
+      map_group_zero_or_more_eq (map_group_zero_or_one m) l;
+      map_group_zero_or_more_eq m l;
+      Classical.forall_intro prf;
+      bound_map_group_ext l (map_group_zero_or_more (map_group_zero_or_one m)) (map_group_zero_or_more m)
+    )
+    (fun l prf l' ->
+      map_group_zero_or_more_eq (map_group_zero_or_one m) l;
+      map_group_zero_or_more_eq m l;
+      assert (~ (map_group_zero_or_one m l == MapGroupResult FStar.GSet.empty));
+      Classical.forall_intro prf;
+      bound_map_group_ext l (map_group_zero_or_more (map_group_zero_or_one m)) (map_group_zero_or_more m);
+      let (l1, l2) = map_group_concat_elim (map_group_zero_or_one m) (bound_map_group l (map_group_zero_or_more m)) l l' in
+      ()
+    )
+    (fun l prf l' ->
+      map_group_zero_or_more_eq (map_group_zero_or_one m) l;
+      map_group_zero_or_more_eq m l;
+      assert (~ (map_group_zero_or_one m l == MapGroupResult FStar.GSet.empty));
+      Classical.forall_intro prf;
+      bound_map_group_ext l (map_group_zero_or_more (map_group_zero_or_one m)) (map_group_zero_or_more m);
+      match gset_is_empty (MapGroupResult?._0 (m l)) with
+      | None ->
+        assert (map_group_concat_witness_pred (map_group_zero_or_one m) (bound_map_group l (map_group_zero_or_more m)) l l'
+          (
+            (ghost_map_empty, l),
+            (ghost_map_empty, l)
+          )
+        )
+      | _ -> 
+        let (l1, l2) = map_group_concat_elim m (bound_map_group l (map_group_zero_or_more m)) l l' in
+        ()
+    )
+
+let apply_map_group_det_old (m: map_group) (l: cbor_map) : Pure map_group_result
+  (requires True)
+  (ensures fun r -> map_group_result_prop l r)
+= match m l with
+  | MapGroupCutFailure -> MapGroupCutFail
+  | MapGroupResult s ->
+  if FStar.StrongExcludedMiddle.strong_excluded_middle (s == FStar.GSet.empty)
+  then MapGroupFail
+  else if FStar.StrongExcludedMiddle.strong_excluded_middle (exists x . s == FStar.GSet.singleton x)
+  then
+    let x = FStar.IndefiniteDescription.indefinite_description_ghost _ (fun x -> s == FStar.GSet.singleton x) in
+    MapGroupDet (fst x) (snd x)
+  else MapGroupNonDet
+
+let gset_is_singleton (#t: Type) (s: FStar.GSet.set t) (x: t) : Tot prop =
+  s == FStar.GSet.singleton x
+
+let apply_map_group_det (m: map_group) (l: cbor_map) : Pure map_group_result
+  (requires True)
+  (ensures fun r -> map_group_result_prop l r)
+= match m l with
+  | MapGroupCutFailure -> MapGroupCutFail
+  | MapGroupResult s ->
+  begin match gset_is_empty s with
+  | None -> MapGroupFail
+  | _ ->
+    begin match maybe_indefinite_description_ghost (gset_is_singleton s) with
+    | Some x -> MapGroupDet (fst x) (snd x)
+    | _ -> MapGroupNonDet
+    end
+  end
+
+let apply_map_group_det_eq_old
+  (m: map_group)
+  (l: cbor_map)
+: Lemma
+  (apply_map_group_det m l == apply_map_group_det_old m l)
+= ()
+
+#restart-solver
+let apply_map_group_det_eq_singleton (m: map_group) (l: cbor_map) (x : (_ & _)) : Lemma
+  (requires (match m l with
+  | MapGroupResult s -> s `FStar.GSet.equal` FStar.GSet.singleton x
+  | _ -> False
+  ))
+  (ensures (apply_map_group_det m l == MapGroupDet (fst x) (snd x)))
+= let MapGroupResult s = m l in
+  assert (s == FStar.GSet.singleton x);
+  if FStar.StrongExcludedMiddle.strong_excluded_middle (s == FStar.GSet.empty)
+  then assert (x `FStar.GSet.mem` FStar.GSet.empty)
+  else begin
+    assert (exists x . s == FStar.GSet.singleton x);
+    assert (MapGroupDet? (apply_map_group_det m l))
+  end
+
+#restart-solver
+let apply_map_group_det_eq_map (m1 m2: map_group) (l: cbor_map) : Lemma
+  (requires m1 l == m2 l)
+  (ensures apply_map_group_det m1 l == apply_map_group_det m2 l)
+= match apply_map_group_det m1 l with
+  | MapGroupDet c1 l1 -> apply_map_group_det_eq_singleton m2 l (c1, l1)
+  | _ -> ()
+
+let apply_map_group_det_always_false (l: cbor_map) : Lemma
+  (apply_map_group_det map_group_always_false l == MapGroupFail)
+= ()
+
+#restart-solver
+let apply_map_group_det_nop (l: cbor_map) : Lemma
+  (apply_map_group_det map_group_nop l == MapGroupDet ghost_map_empty l)
+= ()
+
+let apply_map_group_det_end l = ()
+
+let apply_map_group_det_map_group_equiv (m1 m2: map_group) : Lemma
+  (requires
+    (forall l . ~ (MapGroupNonDet? (apply_map_group_det m1 l))) /\
+    (forall l . apply_map_group_det m1 l == apply_map_group_det m2 l)
+  )
+  (ensures m1 == m2)
+= map_group_equiv_intro m1 m2
+    (fun l -> ())
+    (fun l l' ->
+      let MapGroupDet _ s1 = apply_map_group_det m1 l in
+      let (k1, l1) = FStar.IndefiniteDescription.indefinite_description_ghost _ (fun s1 -> m1 l == MapGroupResult (FStar.GSet.singleton s1)) in
+      let (k2, l2) = FStar.IndefiniteDescription.indefinite_description_ghost _ (fun s2 -> m2 l == MapGroupResult (FStar.GSet.singleton s2)) in
+      assert (l1 == l2);
+      ghost_map_equiv k1 k2
+    )
+    (fun l l' ->
+      let MapGroupDet _ s1 = apply_map_group_det m1 l in
+      let (k1, l1) = FStar.IndefiniteDescription.indefinite_description_ghost _ (fun s1 -> m1 l == MapGroupResult (FStar.GSet.singleton s1)) in
+      let (k2, l2) = FStar.IndefiniteDescription.indefinite_description_ghost _ (fun s2 -> m2 l == MapGroupResult (FStar.GSet.singleton s2)) in
+      assert (l1 == l2);
+      ghost_map_equiv k1 k2
+    )
+
+let gset_singleton_inj
+  (#t: Type)
+  (x1 x2: t)
+: Lemma
+  (requires FStar.GSet.singleton x1 == FStar.GSet.singleton x2)
+  (ensures x1 == x2)
+= assert (x1 `FStar.GSet.mem` FStar.GSet.singleton x2)
+
+#restart-solver
+let apply_map_group_det_choice (m1 m2: map_group) (l: cbor_map)
+= match apply_map_group_det m1 l with
+  | MapGroupFail -> apply_map_group_det_eq_map (m1 `map_group_choice` m2) m2 l
+  | _ -> apply_map_group_det_eq_map (m1 `map_group_choice` m2) m1 l
+
+val apply_map_group_det_old_concat (m1 m2: map_group) (l: ghost_map Cbor.raw_data_item Cbor.raw_data_item) : Lemma
+  (match apply_map_group_det_old m1 l with
+  | MapGroupCutFail -> apply_map_group_det_old (m1 `map_group_concat` m2) l == MapGroupCutFail
+  | MapGroupFail -> apply_map_group_det_old (m1 `map_group_concat` m2) l == MapGroupFail
+  | MapGroupDet c1 l1 ->
+    apply_map_group_det_old (m1 `map_group_concat` m2) l == begin match apply_map_group_det_old m2 l1 with
+    | MapGroupDet c2 l2 -> MapGroupDet (c1 `ghost_map_union` c2) l2
+    | res -> res
+    end
+  | _ -> True)
+
+#push-options "--z3rlimit 32"
+
+#restart-solver
+let apply_map_group_det_old_concat (m1 m2: map_group) (l: cbor_map)
+= match apply_map_group_det_old m1 l with
+  | MapGroupCutFail -> ()
+  | MapGroupFail ->
+    assert (m1 l == MapGroupResult FStar.GSet.empty);
+    assert (forall x . ~ (FStar.GSet.mem x (MapGroupResult?._0 (m1 l))));
+    assert (match map_group_concat m1 m2 l with
+    | MapGroupResult s -> s `FStar.GSet.equal` FStar.GSet.empty
+    | _ -> False)
+  | MapGroupDet c1 lr1 ->
+    let l1 = FStar.IndefiniteDescription.indefinite_description_ghost _ (fun x -> m1 l == MapGroupResult (FStar.GSet.singleton x)) in
+    assert ((c1, lr1) `FStar.GSet.mem` FStar.GSet.singleton l1);
+    begin match apply_map_group_det_old m2 lr1 with
+    | MapGroupCutFail -> assert (map_group_concat_cut_failure_witness_pred m1 m2 l l1)
+    | MapGroupFail -> assert (match map_group_concat m1 m2 l with
+    | MapGroupResult s -> s `FStar.GSet.equal` FStar.GSet.empty
+    | _ -> False)
+    | MapGroupDet c2 lr2 ->
+      let l2 = FStar.IndefiniteDescription.indefinite_description_ghost _ (fun x -> m2 lr1 == MapGroupResult (FStar.GSet.singleton x)) in
+      assert ((c2, lr2) `FStar.GSet.mem` FStar.GSet.singleton l2);
+      let l0 = (ghost_map_union (fst l1) (fst l2), snd l2) in
+      gset_equal_intro
+        (MapGroupResult?._0 (map_group_concat m1 m2 l))
+        (FStar.GSet.singleton l0)
+        (fun _ -> ())
+        (fun _ ->
+          assert (map_group_concat_witness_pred m1 m2 l l0
+            (l1, l2)
+          )
+        );
+      assert (map_group_concat m1 m2 l == MapGroupResult (FStar.GSet.singleton l0));
+      assert (fst l1 == c1);
+      assert (fst l2 == c2);
+      assert (snd l2 == lr2)
+    | MapGroupNonDet ->
+      let Some l2 = gset_is_empty (MapGroupResult?._0 (m2 lr1)) in
+      let l0 = (ghost_map_union (fst l1) (fst l2), snd l2) in
+      assert (map_group_concat_witness_pred m1 m2 l l0
+        (l1, l2)
+      );
+      assert (FStar.GSet.mem l0 (MapGroupResult?._0 (map_group_concat m1 m2 l)));
+      assert (~ (map_group_concat m1 m2 l == MapGroupResult FStar.GSet.empty));
+      if FStar.StrongExcludedMiddle.strong_excluded_middle (exists x . map_group_concat m1 m2 l == MapGroupResult (FStar.GSet.singleton x))
+      then begin
+        assert (match map_group_concat m1 m2 l with
+        |  MapGroupResult s -> s `FStar.GSet.equal` FStar.GSet.singleton l0
+        | _ -> False);
+        gset_equal_intro
+          (MapGroupResult?._0 (m2 lr1))
+          (FStar.GSet.singleton l2)
+          (fun l2' ->
+            let l0' = (ghost_map_union (fst l1) (fst l2'), snd l2') in
+            assert (map_group_concat_witness_pred m1 m2 l l0'
+              (l1, l2')
+            );
+            assert (FStar.GSet.mem l0' (MapGroupResult?._0 (map_group_concat m1 m2 l)));
+            assert (l0' == l0);
+            ghost_map_disjoint_mem_union' (fst l1) (fst l2') ();
+            ghost_map_disjoint_mem_union' (fst l1) (fst l2) ();
+            ghost_map_equiv (fst l2') (fst l2);
+            assert (l2' == l2)
+          )
+          (fun _ -> ())
+      end
+      else ()
+    end
+  | _ -> ()
+
+#pop-options
+
+let apply_map_group_det_concat (m1 m2: map_group) (l: cbor_map) =
+  apply_map_group_det_old_concat m1 m2 l
+
+#restart-solver
+let apply_map_group_det_match_item_for
+  (cut: bool)
+  (k: Cbor.raw_data_item)
+  (ty: typ)
+  (l: cbor_map)
+= map_group_match_item_for_eq_gen cut k ty l;
+  match apply_ghost_map l k with
+  | Some v ->
+    if ty v
+    then begin
+      let l1 = ghost_map_singleton k v in
+      let l2 = ghost_map_filter (notp_g (matches_map_group_entry (t_literal k) ty)) l in
+      ghost_map_equiv
+        (l `ghost_map_sub` l1)
+        l2;
+      let MapGroupResult s = map_group_match_item_for cut k ty l in
+      assert (gset_is_singleton s (l1, l2));
+      let Some l' = maybe_indefinite_description_ghost (gset_is_singleton s) in
+      gset_singleton_inj l' (l1, l2)
+    end
+    else ()
+  | _ -> ()
+
+// FIXME: swap `notp f` with `f`?
+let map_group_filter_item
+  (f: (Cbor.raw_data_item & Cbor.raw_data_item) -> GTot bool)
+  (l: cbor_map)
+: GTot (cbor_map & cbor_map)
+=
+  ghost_map_filter (notp_g f) l,
+  ghost_map_filter f l
+
+let map_group_item_post_filter
+  (f: (Cbor.raw_data_item & Cbor.raw_data_item) -> GTot bool)
+  (l: cbor_map)
+: Lemma
+  (map_group_item_post l (map_group_filter_item f l))
+  [SMTPat (map_group_filter_item f l)]
+= ghost_map_split f l
+
+let map_group_filter
+  f
+= FE.on_dom_g cbor_map #map_group_codom (fun l ->
+    MapGroupResult (FStar.GSet.singleton (map_group_filter_item f l))
+  )
+
+let apply_map_group_det_filter
+  f l
+= apply_map_group_det_eq_singleton (map_group_filter f) l (map_group_filter_item f l)
+
+let orp_g (#t: Type) (p1 p2: t -> GTot bool) (x: t) : GTot bool =
+  p1 x || p2 x
+
+let ghost_map_filter_union
+  (#key #value: Type)
+  (p1 p2: (key & value) -> GTot bool)
+  (m: ghost_map key value)
+: Lemma
+  (ghost_map_filter p1 m `ghost_map_union`
+    ghost_map_filter p2 m ==
+    ghost_map_filter (p1 `orp_g` p2) m
+  )
+= ghost_map_ext
+    (ghost_map_filter p1 m `ghost_map_union`
+      ghost_map_filter p2 m)
+    (ghost_map_filter (p1 `orp_g` p2) m)
+
+let ghost_map_filter_not_filter_not_strong
+  (p1 p2: (Cbor.raw_data_item & Cbor.raw_data_item) -> GTot bool)
+  (l: cbor_map)
+: Lemma
+  (ghost_map_filter (notp_g p1) l `ghost_map_union`
+    ghost_map_filter (notp_g p2) (ghost_map_filter p1 l) ==
+    ghost_map_filter (notp_g (p1 `andp_g` p2)) l
+  )
+= ghost_map_filter_filter p1 (notp_g p2) l;
+  ghost_map_filter_union (notp_g p1) (p1 `andp_g` notp_g p2) l;
+  ghost_map_filter_ext
+    (notp_g p1 `orp_g` (p1 `andp_g` notp_g p2))
+    (notp_g (p1 `andp_g` p2))
+    l
+
+let map_group_filter_filter
+  p1 p2
+= Classical.forall_intro (ghost_map_filter_filter p1 p2);
+  Classical.forall_intro (ghost_map_filter_not_filter_not_strong p1 p2);
+  apply_map_group_det_map_group_equiv
+    (map_group_filter p1 `map_group_concat` map_group_filter p2)
+    (map_group_filter (andp_g p1 p2))
+
+#restart-solver
+let map_group_zero_or_one_match_item_filter_matched
+  (key value: typ)
+  (p: (Cbor.raw_data_item & Cbor.raw_data_item) -> GTot bool)
+  (l: cbor_map)
+  kv l'
+: Lemma
+  (requires (
+    (forall x . p x ==> notp_g (matches_map_group_entry key value) x) /\
+    map_group_item_post l (ghost_map_singleton (fst kv) (snd kv), l') /\
+    matches_map_group_entry key value kv
+  ))
+  (ensures (
+    ghost_map_singleton (fst kv) (snd kv) `ghost_map_union` ghost_map_filter (notp_g p) l' ==
+      ghost_map_filter (notp_g p) l /\
+    ghost_map_filter p l' ==
+      ghost_map_filter p l
+  ))
+= let s = ghost_map_singleton (fst kv) (snd kv) in
+  ghost_map_disjoint_union_filter (notp_g p) s l';
+  ghost_map_equiv s (ghost_map_filter (notp_g p) s);
+  ghost_map_disjoint_union_filter p s l';
+  ghost_map_equiv ghost_map_empty (ghost_map_filter p s)
+
+#restart-solver
+let map_group_zero_or_one_match_item_filter
+  key value p
+= map_group_equiv_intro
+    (map_group_zero_or_one (map_group_match_item false key value) `map_group_concat` map_group_filter p)
+    (map_group_filter p)
+    (fun _ -> ())
+    (fun l l' ->
+      let MapGroupResult s = map_group_match_item false key value l in
+      match gset_is_empty s with
+      | None -> map_group_concat_nop_l (map_group_filter p)
+      | Some _ ->
+        let (l1, _) = map_group_concat_elim (map_group_zero_or_one (map_group_match_item false key value)) (map_group_filter p) l l' in
+        let kv = map_group_match_item_elim key value l l1 in
+        assert (fst l1 == ghost_map_singleton (fst kv) (snd kv));
+        assert (map_group_filter p (snd l1) == MapGroupResult (FStar.GSet.singleton (map_group_filter_item p (snd l1))));
+        map_group_zero_or_one_match_item_filter_matched key value p l kv (snd l1);
+        assert (snd l' == ghost_map_filter p l)
+    )
+    (fun l l' ->
+      let MapGroupResult s = map_group_match_item false key value l in
+      match gset_is_empty s with
+      | None -> map_group_concat_nop_l (map_group_filter p)
+      | Some l1 ->
+        let kv = map_group_match_item_elim key value l l1 in
+        map_group_zero_or_one_match_item_filter_matched key value p l kv (snd l1);
+        assert (map_group_concat_witness_pred (map_group_zero_or_one (map_group_match_item false key value)) (map_group_filter p) l l' (l1, (ghost_map_filter (notp_g p) (snd l1), ghost_map_filter p (snd l1))))
+    )
+
+#push-options "--z3rlimit 32"
+
+#restart-solver
+let map_group_concat_bound_map_group_elim
+  (m1 m2: map_group)
+  (l1 l2: cbor_map)
+  (prf: (l': _) -> Lemma
+    (requires (match m1 l1 with
+    | MapGroupResult s -> FStar.GSet.mem l' s
+    | _ -> False
+    ))
+    (ensures (ghost_map_length (snd l') < ghost_map_length l2))
+  )
+: Lemma
+  ((m1 `map_group_concat` bound_map_group l2 m2) l1 ==
+    (m1 `map_group_concat` m2) l1)
+= Classical.forall_intro (Classical.move_requires prf);
+  match m1 l1 with
+  | MapGroupCutFailure -> ()
+  | MapGroupResult s ->
+    begin match (m1 `map_group_concat` bound_map_group l2 m2) l1, (m1 `map_group_concat` m2) l1 with
+    | MapGroupResult s, MapGroupResult s' -> assert (s `FStar.GSet.equal` s')
+    | _ -> ()
+    end
+
+#pop-options
+
+let map_group_concat_eq_l
+  (m1 m1' m2: map_group)
+  (l: cbor_map)
+: Lemma
+  (requires (
+    m1 l == m1' l
+  ))
+  (ensures (
+    (m1 `map_group_concat` m2) l ==
+      (m1' `map_group_concat` m2) l
+  ))
+= match (m1 `map_group_concat` m2) l, (m1' `map_group_concat` m2) l with
+  | MapGroupResult s, MapGroupResult s' -> assert (s `FStar.GSet.equal` s')
+  | _ -> ()
+
+#restart-solver
+let map_group_zero_or_one_bound_match_item_filter
+  (key value: typ)
+  (l: cbor_map)
+: Lemma
+  (ensures (
+    let p = notp_g (matches_map_group_entry key value) in
+    (map_group_zero_or_one (map_group_match_item false key value) `map_group_concat` bound_map_group l (map_group_filter p)) l == map_group_filter p l
+  ))
+= let p = notp_g (matches_map_group_entry key value) in
+  map_group_match_item_alt_correct key value l;
+  match maybe_indefinite_description_ghost (map_group_match_item_alt_pred key value l) with
+  | None ->
+    map_group_concat_eq_l (map_group_zero_or_one (map_group_match_item false key value)) map_group_nop (bound_map_group l (map_group_filter p)) l;
+    map_group_concat_nop_l (bound_map_group l (map_group_filter p));
+    ghost_map_equiv
+      (ghost_map_filter (notp_g p) l)
+      ghost_map_empty;
+    ghost_map_equiv
+      (ghost_map_filter p l)
+      l
+  | Some _ ->
+    assert (Some? (gset_is_empty (map_group_match_item' key value l)));
+    map_group_concat_bound_map_group_elim
+      (map_group_zero_or_one (map_group_match_item false key value))
+      (map_group_filter p)
+      l l
+      (fun _ -> ());
+    map_group_zero_or_one_match_item_filter key value p
+
+#restart-solver
+let map_group_zero_or_one_map_group_match_item_no_cut_nonempty
+  (key value: typ)
+  (l: cbor_map)
+: Lemma
+  (~ (map_group_zero_or_one (map_group_match_item false key value) l == MapGroupResult FStar.GSet.empty))
+= let MapGroupResult s = map_group_match_item false key value l in
+  let MapGroupResult s' = map_group_zero_or_one (map_group_match_item false key value) l in
+  match gset_is_empty s with
+  | None -> assert (FStar.GSet.mem (ghost_map_empty, l) s')
+  | _ -> ()
+
+#push-options "--z3rlimit 16"
+
+#restart-solver
+let map_group_zero_or_more_match_item_filter (key value: typ) : Lemma
+  (ensures
+    map_group_zero_or_more (map_group_match_item false key value) == map_group_filter (notp_g (matches_map_group_entry key value))
+  )
+= let f = (notp_g (matches_map_group_entry key value)) in
+  map_group_equiv_intro_equiv_rec
+    (map_group_zero_or_more (map_group_match_item false key value))
+    (map_group_filter (notp_g (matches_map_group_entry key value)))
+    (fun l prf ->
+      map_group_zero_or_more_zero_or_one_eq (map_group_match_item false key value);
+      map_group_zero_or_more_eq (map_group_zero_or_one (map_group_match_item false key value)) l;
+      map_group_zero_or_one_map_group_match_item_no_cut_nonempty key value l;
+      Classical.forall_intro prf    
+    )
+    (fun l prf l' ->
+      map_group_zero_or_more_zero_or_one_eq (map_group_match_item false key value);
+      map_group_zero_or_more_eq (map_group_zero_or_one (map_group_match_item false key value)) l;
+      map_group_zero_or_one_map_group_match_item_no_cut_nonempty key value l;
+      Classical.forall_intro prf;
+      bound_map_group_ext l (map_group_zero_or_more (map_group_match_item false key value)) (map_group_filter f);
+      map_group_zero_or_one_bound_match_item_filter key value l
+    )
+
+#pop-options
+
+#restart-solver
+let apply_map_group_det_zero_or_more_match_item
+  (key value: typ)
+  (l: cbor_map)
+= map_group_zero_or_more_match_item_filter key value;
+  ghost_map_filter_ext
+    (matches_map_group_entry key value)
+    (notp_g (notp_g (matches_map_group_entry key value)))
+    l;
+  apply_map_group_det_eq_singleton (map_group_zero_or_more (map_group_match_item false key value)) l
+    (
+      ghost_map_filter (matches_map_group_entry key value) l,
+      ghost_map_filter (notp_g (matches_map_group_entry key value)) l
+    )
+
+(*
+#push-options "--z3rlimit 64"
+
+#restart-solver
+let map_group_zero_or_more_map_group_match_item_for
+  (key: Cbor.raw_data_item)
+  (value: typ)
+: Lemma
+  (map_group_zero_or_more (map_group_match_item_for false key value) ==
+    map_group_zero_or_one (map_group_match_item_for false key value)
+  )
+= apply_map_group_det_map_group_equiv0
+    (map_group_zero_or_more (map_group_match_item_for false key value))
+    (map_group_zero_or_one (map_group_match_item_for false key value))
+    (fun l -> ())
+    (fun l ->
+      Classical.move_requires (list_ghost_assoc_none_filter_matches_map_group_entry_for key value) l;
+      let MapGroupDet c1 _ = apply_map_group_det (map_group_zero_or_more (map_group_match_item_for false key value)) l in
+      let MapGroupDet c2 _ = apply_map_group_det (map_group_zero_or_one (map_group_match_item_for false key value)) l in
+      assert (c1 `ghost_map_feq` c2)
+    )
+
+#pop-options
+
+let map_group_choice_assoc
+  (g1 g2 g3: map_group)
+: Lemma
+  ((g1 `map_group_choice` g2) `map_group_choice` g3 == g1 `map_group_choice` (g2 `map_group_choice` g3))
+= assert (((g1 `map_group_choice` g2) `map_group_choice` g3) `map_group_equiv` (g1 `map_group_choice` (g2 `map_group_choice` g3)))
+
+let map_group_zero_or_one_choice
+  (g1 g2: map_group)
+: Lemma
+  (map_group_zero_or_one (g1 `map_group_choice` g2) == g1 `map_group_choice` map_group_zero_or_one g2)
+= map_group_choice_assoc g1 g2 map_group_nop
+
+let matches_map_group (g: map_group) (m: cbor_map) : GTot bool =
+  MapGroupResult? (g m) &&
+  FStar.StrongExcludedMiddle.strong_excluded_middle (exists gm .
+    FStar.GSet.mem (gm, []) (MapGroupResult?._0 (g m))
+  )
+
+let matches_map_group_mem (g: map_group) (m: cbor_map) (gm: _) : Lemma
+  (requires (match g m with
+  | MapGroupResult s -> FStar.GSet.mem (gm, []) s
+  | _ -> False
+  ))
+  (ensures gm == ghost_map_of_list m)
+  [SMTPat (FStar.GSet.mem (gm, []) (MapGroupResult?._0 (g m)))]
+= Classical.forall_intro (ghost_map_of_list_mem m);
+  ghost_map_equiv gm (ghost_map_of_list m)
+
+let matches_map_group_det (g: map_group) (m: cbor_map) : Lemma
+  (match apply_map_group_det g m with
+  | MapGroupCutFail
+  | MapGroupFail -> ~ (matches_map_group g m)
+  | MapGroupDet _ m' -> matches_map_group g m <==> m' == []
+  | _ -> True)
+= ()
